\documentclass{article}
\usepackage{amsmath}
\usepackage[round]{natbib}

\begin{document}

\newcommand{\jj}{\sqrt{1+\left(y'\right)^2}}
\section*{Abstract}
In this short article I discuss skipping ropes



\section{Introduction}

The dynamics of skipping ropes is an everyday yet fascinating topic.
Here I analyse the dynamics of a slowly rotating skipper.



\citep{mohazzabi1999}


With arclength $s$ and Cartesian $(x,y)$ coordinates and [possibly
  nonconservative] force field

\begin{equation}
  \begin{bmatrix}F\\G\end{bmatrix}
    =
    \begin{bmatrix}F(x,y)\\G(x,y)\end{bmatrix}
\end{equation}
and tensions $T,U$ [formerly $T_x,T_y$] we get

\begin{eqnarray}
  \frac{dT}{dx}=-F\jj\label{Tx}\\
  \frac{dU}{dx}=-G\jj\label{Ty}
  \end{eqnarray}

\begin{equation}
  \frac{U}{T}=\frac{dy}{dx}=y'
\end{equation}

So (writing $T_x=T$ for convenience)

\begin{equation}
U'=(y'T)'=y''T+y'T'=-G\jj
\end{equation}

Solving for $T$:

\begin{eqnarray}
  T &=& -(y'')^{-1}\left[G\jj + y'T'\right]\nonumber\\
  &=& -(y'')^{-1}\left[G\jj -y'F\jj\right]\nonumber\\
    &=& (y'')^{-1}\jj(y'F-G)\label{eqforT}
\end{eqnarray}

Differentiating equation~\ref{eqforT}:

\begin{eqnarray}
  T'&=& \left[(y'')^{-1}\jj(y'F-G)\right]'\nonumber\\
  &=& -(y'')^{-2}y'''\jj\left[y'F-G\right]\nonumber\\
  &{}& \qquad +\frac{y'}{\jj}(y'F-G)\nonumber\\
  &{}& \quad\quad + (y'')^{-1}\jj\left[y'F-G\right]'
\end{eqnarray}

Now we use the fact that $F'=F_x+y'F_y$ and $G'=G_x+y'G_y$ (where
subscripts denote partial differentials).  This gives
$\left[y'F-G\right]'=y''F+y'F_x+(y')^2F_y-G_x-y'G_y$ so

\begin{eqnarray}
 T' &=& -(y'')^{-2}y'''\jj\left(y'F-G\right)\nonumber\\
  &{}&\quad +\frac{y'}{\jj}(y'F-G)\nonumber\\
 &{}& \quad\quad+(y'')^{-1}\jj
 \left( y''F+y'F_x+(y')^2F_y-G_x-y'G_y \right)
\end{eqnarray}

Substituting for $T'$ from equation~\ref{Tx} we get

\begin{eqnarray}
  (y'')^{-2}y'''\jj(y'F-G)=&+&F\jj\nonumber\\
  &+&\frac{y'}{\jj}(y'F-G)\\
  &+&(y'')^{-1}\jj\left(y''F+y'F_x+(y')^2F_y-G_x-y'G_y  \right)
  \nonumber
\end{eqnarray}
  

Solving for $y'''$ and simplifying gives
\begin{eqnarray}
  y'''&=&\frac{(y'')^2F}{y'F-G}
  + \frac{y'(y'')^2}{1+(y')^2}
  + \frac{y''\left(y''F+y'F_x+(y')^2F_y-G_x-y'G_y \right)}{y'F-G}\\
 &=&
   \frac{y'(y'')^2}{1+(y')^2}
  + \frac{y''\left(2y''F+y'F_x-G_x\right)}{y'F-G}
\end{eqnarray}

As a consistency check if we have $F=0,G=-1$ [corresponding to a
  uniform vertical gravitational field], we would have

\begin{equation}
  y'''=\frac{y'(y'')^2}{1+(y')^2}
\end{equation}

which is satisfied by $y=a\cosh(x/a)$, the standard equation for a
catenary.  Further, if $F=-1,G=0$ [corresponding to a horizontal
  gravitational field] we would have

\begin{equation}
  y''' = \frac{y'(y'')^2\left(y''\right)^2}{1+(y')^2}-\frac{2y''}{y'}
\end{equation}

satisfied by $y=a\operatorname{arcosh}(x/a)$.

\bibliography{skipping}
\bibliographystyle{plainnat}
\end{document}
